Made decode_bitwise proofs go away, and proved sane lemmas about Z.testbit (BaseSystem.decode _ _)

src/ModularArithmetic/Pow2BaseProofs.v
@@ -12,6 +12,36 @@ Local Open Scope Z_scope.
 
 Create HintDb simpl_add_to_nth discriminated.
 
+(* TODO : move to ZUtil *)
+  Lemma ones_spec : forall n m, 0 <= n -> 0 <= m -> Z.testbit (Z.ones n) m = if Z_lt_dec m n then true else false.
+  Proof.
+    intros.
+    break_if.
+    + apply Z.ones_spec_low. omega.
+    + apply Z.ones_spec_high. omega.
+  Qed.
+
+(* TODO : move to ZUtil *)
+Create HintDb Ztestbit discriminated.
+Hint Rewrite Z.land_spec Z.lor_spec Z.shiftl_spec Z.shiftr_spec ones_spec using omega : Ztestbit.
+Hint Rewrite Z.testbit_neg_r using omega : Ztestbit.
+Hint Rewrite Bool.andb_true_r Bool.andb_false_r Bool.orb_true_r Bool.orb_false_r
+            Bool.andb_true_l Bool.andb_false_l Bool.orb_true_l Bool.orb_false_l : Ztestbit.
+
+(* TODO : move *)
+Lemma testbit_pow2_mod : forall a n i, 0 <= i ->  0 <= n ->
+Z.testbit (Z.pow2_mod a n) i = if Z_lt_dec i n then Z.testbit a i else false.
+Proof.
+cbv [Z.pow2_mod]; intros.
+repeat match goal with
+        | |- _ => break_if
+        | |- _ => omega
+        | |- _ => reflexivity
+        | |- _ => progress autorewrite with Ztestbit
+        end.
+Qed.
+Hint Rewrite testbit_pow2_mod using omega : Ztestbit.
+
 Section Pow2BaseProofs.
   Context {limb_widths} (limb_widths_nonneg : forall w, In w limb_widths -> 0 <= w).
   Local Notation base := (base_from_limb_widths limb_widths).
@@ -170,20 +200,6 @@ Section Pow2BaseProofs.
   Proof.
   Admitted.
 
-  Lemma ones_spec : forall n m, 0 <= n -> 0 <= m -> Z.testbit (Z.ones n) m = if Z_lt_dec m n then true else false.
-  Proof.
-    intros.
-    break_if.
-    + apply Z.ones_spec_low. omega.
-    + apply Z.ones_spec_high. omega.
-  Qed.
-
-  Create HintDb Ztestbit.
-  Hint Rewrite Z.land_spec Z.lor_spec Z.shiftl_spec Z.shiftr_spec ones_spec using omega : Ztestbit.
-  Hint Rewrite Z.testbit_neg_r using omega : Ztestbit.
-  Hint Rewrite Bool.andb_true_r Bool.andb_false_r Bool.orb_true_r Bool.orb_false_r
-               Bool.andb_true_l Bool.andb_false_l Bool.orb_true_l Bool.orb_false_l : Ztestbit.
-
   (* TODO : move *)
   Lemma pow2_mod_split : forall a n m, 0 <= n -> 0 <= m ->
                                        Z.pow2_mod a (n + m) = Z.lor (Z.pow2_mod a n) ((Z.pow2_mod (a >> n) m) << n).
@@ -196,9 +212,6 @@ Section Pow2BaseProofs.
     autorewrite with Ztestbit; reflexivity.
   Qed.
 
-  Lemma decode_firstn_succ : forall us i, BaseSystem.decode base (firstn (S i) us) =
-    BaseSystem.decode base (firstn i us) + (nth_default 0 us i << sum_firstn limb_widths i).
-  Admitted.
 
   (* TODO : move *)
   Lemma pow2_mod_pow2_mod : forall a n m, 0 <= n -> 0 <= m ->
@@ -231,6 +244,7 @@ Section Pow2BaseProofs.
     clear limb_widths limb_widths_nonneg.
   Admitted.
 
+  
   (* TODO : move *)
   Lemma pow2_mod_add_shiftl_low : forall a b n m, m <= n -> Z.pow2_mod (a + b << n) m = Z.pow2_mod a m.
   Proof.
@@ -296,6 +310,143 @@ Section Pow2BaseProofs.
           repeat f_equal; try ring.
   Qed.
 
+  Lemma nth_default_limb_widths_nonneg : forall i, 0 <= nth_default 0 limb_widths i.
+  Proof.
+    intros; apply nth_default_preserves_properties; auto; omega.
+  Qed. Hint Resolve nth_default_limb_widths_nonneg.
+
+  Lemma decode_firstn_pow2_mod : forall us i,
+    (i <= length us)%nat ->
+    length us = length limb_widths ->
+    bounded limb_widths us ->
+    BaseSystem.decode' base (firstn i us) = Z.pow2_mod (BaseSystem.decode' base us) (sum_firstn limb_widths i).
+  Proof.
+    intros; induction i;
+    repeat match goal with
+           | |- _ => rewrite firstn_0, sum_firstn_0, decode_nil, pow2_mod_0_r; reflexivity
+           | |- _ => progress distr_length
+           | |- _ => rewrite firstn_succ with (d := 0)
+           | |- _ => rewrite set_higher
+           | |- _ => rewrite nth_default_base
+           | |- _ => rewrite IHi
+           | |- _ => rewrite <-Z.lor_shiftl by (rewrite ?Z.pow2_mod_spec; try apply Z.mod_pos_bound; zero_bounds)
+           | |- appcontext[Nat.min ?x ?y] => (rewrite Nat.min_l by omega || rewrite Nat.min_r by omega)
+           | |- appcontext[2 ^ ?a * _] => rewrite (Z.mul_comm (2 ^ a)); rewrite <-Z.shiftl_mul_pow2
+           | |- _ => solve [auto]
+           | |- _ => lia
+           end.
+    rewrite digit_select by assumption; apply Z.bits_inj'.
+    repeat match goal with
+           | |- _ => progress intros
+           | |- _ => progress autorewrite with Ztestbit
+           | |- _ => rewrite testbit_pow2_mod by (omega || trivial)
+           | |- _ => break_if; try omega
+           | H : ?a < ?b |- appcontext[Z.testbit _ (?a - ?b)] =>
+             rewrite (Z.testbit_neg_r _ (a-b)) by omega
+           | |- _ => reflexivity
+           | |- _ => solve [f_equal; ring]
+           | |- _ => rewrite sum_firstn_succ_default in *;
+                       pose proof (nth_default_limb_widths_nonneg i); omega
+           end.
+  Qed.
+
+  Lemma testbit_decode_firstn_high : forall us i n,
+    (i <= length us)%nat ->
+    length us = length limb_widths ->
+    bounded limb_widths us ->
+    sum_firstn limb_widths i <= n ->
+    Z.testbit (BaseSystem.decode base (firstn i us)) n = false.
+  Proof.
+    repeat match goal with
+           | |- _ => progress intros
+           | |- _ => progress autorewrite with Ztestbit
+           | |- _ => rewrite decode_firstn_pow2_mod
+           | |- _ => rewrite testbit_pow2_mod
+           | |- _ => break_if
+           | |- _ => assumption
+           | |- _ => solve [auto] 
+           | H : ?a <= ?b |- 0 <= ?b => assert (0 <= a) by (omega || auto); omega
+           end.
+  Qed.
+
+  Lemma testbit_decode_high : forall us n,
+    length us = length limb_widths ->
+    bounded limb_widths us ->
+    sum_firstn limb_widths (length us) <= n ->
+    Z.testbit (BaseSystem.decode base us) n = false.
+  Proof.
+    intros.
+    erewrite <-(firstn_all _ us) by reflexivity.
+    auto using testbit_decode_firstn_high.
+  Qed.
+
+  Lemma decode_firstn_succ : forall us i,
+      (S i <= length us)%nat ->
+      bounded limb_widths us ->
+      length us = length limb_widths ->
+      BaseSystem.decode base (firstn (S i) us) =
+      Z.lor (BaseSystem.decode base (firstn i us)) (nth_default 0 us i << sum_firstn limb_widths i).
+  Proof.
+    repeat match goal with
+           | |- _ => progress intros
+           | |- _ => progress autorewrite with Ztestbit
+           | |- _ => progress change BaseSystem.decode with BaseSystem.decode' 
+           | |- _ => rewrite sum_firstn_succ_default in * 
+           | |- _ => apply Z.bits_inj'
+           | |- _ => break_if
+           | |- appcontext [Z.testbit _ (?a - sum_firstn ?l ?i)] =>
+                  destruct (Z_le_dec (sum_firstn l i) a);
+                  [ rewrite (testbit_decode_firstn_high _ i a)
+                  | rewrite (Z.testbit_neg_r _ (a - sum_firstn l i))]
+           | |- appcontext [Z.testbit (BaseSystem.decode' _ (firstn ?i _)) _] =>
+                  rewrite (decode_firstn_pow2_mod _ i)
+           | |- _ => rewrite digit_select by auto
+           | |- _ => rewrite testbit_pow2_mod
+           | |- _ => assumption
+           | |- _ => reflexivity
+           | |- _ => omega
+           | |- _ => f_equal; ring
+           | |- _ => solve [auto]
+           | |- _ => solve [zero_bounds]
+           | H : appcontext [nth_default 0 limb_widths ?i] |- _ =>
+             pose proof (nth_default_limb_widths_nonneg i); omega
+           | |- appcontext [nth_default 0 limb_widths ?i] =>
+             pose proof (nth_default_limb_widths_nonneg i); omega
+           end.
+  Qed.
+
+  Lemma testbit_decode_digit_select : forall us n i,
+    bounded limb_widths us ->
+    sum_firstn limb_widths i <= n < sum_firstn limb_widths (S i) ->
+    Z.testbit (BaseSystem.decode base us) n = Z.testbit (nth_default 0 us i) (n - sum_firstn limb_widths i).
+  Proof.
+    repeat match goal with
+           | |- _ => progress intros
+           | |- _ => erewrite digit_select by eauto
+           | |- _ => progress rewrite sum_firstn_succ_default in *
+           | |- _ => progress autorewrite with Ztestbit
+           | |- _ => break_if
+           | |- _ => omega
+           | |- _ => solve [f_equal;ring]
+           end.
+  Qed.
+
+  Lemma testbit_bounded_high : forall i n us, bounded limb_widths us ->
+                                            nth_default 0 limb_widths i <= n ->
+                                            Z.testbit (nth_default 0 us i) n = false.
+  Proof.
+    repeat match goal with
+           | |- _ => progress intros
+           | |- _ => break_if
+           | |- _ => omega
+           | |- _ => reflexivity
+           | |- _ => assumption
+           | |- _ => apply nth_default_limb_widths_nonneg; auto
+           | H : nth_default 0 limb_widths ?i <= ?n |- 0 <= ?n => etransitivity; [ | eapply H]
+           | |- _ => erewrite <-pow2_mod_bounded by eauto; rewrite testbit_pow2_mod
+           end.
+  Qed.
+
   Lemma pow2_mod_decode_last : forall us vs i n,
     (sum_firstn limb_widths i <= n <= sum_firstn limb_widths (S i)) ->
     firstn i us = firstn i vs ->
@@ -347,6 +498,23 @@ Section Pow2BaseProofs.
     Z.pow2_mod (BaseSystem.decode base us >> n) m =
     Z.pow2_mod (nth_default 0 us i >> (n - sum_firstn limb_widths i)) m.
   Admitted.
+
+  Lemma decode_shift : forall us u0, (length (u0 :: us) <= length limb_widths)%nat ->
+    BaseSystem.decode base (u0 :: us) = u0 + ((BaseSystem.decode (base_from_limb_widths (tl limb_widths)) us) << nth_default 0 limb_widths 0).
+  Proof.
+    induction limb_widths; intros;
+      repeat match goal with
+             | |- _ => rewrite base_from_limb_widths_cons, peel_decode
+             | |- _ => rewrite two_p_correct, Z.shiftl_mul_pow2
+             | |- _ => apply Z.add_cancel_l
+             | |- appcontext[tl (_ :: _)] => cbv [tl]
+             | |- appcontext[map (Z.mul ?a) _] => fold (BaseSystem.mul_each a);
+                                                    rewrite <-!mul_each_base, !mul_each_rep
+             | |- _ => progress distr_length
+             | |- _ => progress autorewrite with push_nth_default zsimplify
+             | |- _ => solve [auto using in_eq, Z.mul_comm]
+            end.
+  Qed.
 
   Section make_base_vector.
     Local Notation k := (sum_firstn limb_widths (length limb_widths)).
@@ -435,11 +603,6 @@ Section BitwiseDecodeEncode.
         congruence.
   Qed.
 
-  Lemma nth_default_limb_widths_nonneg : forall i, 0 <= w[i].
-  Proof.
-    intros; apply nth_default_preserves_properties; auto; omega.
-  Qed. Hint Resolve nth_default_limb_widths_nonneg.
-
   Lemma base_upper_bound_compatible : @base_max_succ_divide base upper_bound.
   Proof.
     unfold base_max_succ_divide; intros i lt_Si_length.
@@ -447,14 +610,14 @@ Section BitwiseDecodeEncode.
     rewrite Nat.lt_eq_cases in lt_Si_length; destruct lt_Si_length;
       rewrite !nth_default_base by (omega || auto).
     + erewrite sum_firstn_succ by (eapply nth_error_Some_nth_default with (x := 0); omega).
-      rewrite Z.pow_add_r; auto using sum_firstn_limb_widths_nonneg.
+      rewrite Z.pow_add_r; eauto using sum_firstn_limb_widths_nonneg, nth_default_limb_widths_nonneg.
       apply Z.divide_factor_r.
     + rewrite nth_default_out_of_bounds by (distr_length; omega).
       unfold Pow2Base.upper_bound.
       replace (length limb_widths) with (S (pred (length limb_widths))) by omega.
       replace i with (pred (length limb_widths)) by omega.
       erewrite sum_firstn_succ by (eapply nth_error_Some_nth_default with (x := 0); omega).
-      rewrite Z.pow_add_r; auto using sum_firstn_limb_widths_nonneg.
+      rewrite Z.pow_add_r; eauto using sum_firstn_limb_widths_nonneg, nth_default_limb_widths_nonneg.
       apply Z.divide_factor_r.
   Qed.
   Hint Resolve base_upper_bound_compatible.
@@ -471,126 +634,64 @@ Section BitwiseDecodeEncode.
     reflexivity.
   Qed.
 
-  Lemma decode_bitwise'_nil : forall i,
-    decode_bitwise' limb_widths nil i 0 = 0.
+
+  Definition decode_bitwise'_invariant us i acc :=
+    forall n, 0 <= n -> Z.testbit acc n = Z.testbit (BaseSystem.decode base us) (n + sum_firstn limb_widths i).
+
+  Lemma decode_bitwise'_invariant_step : forall us,
+    length us = length limb_widths ->
+    bounded limb_widths us ->
+    forall i acc, decode_bitwise'_invariant us (S i) acc ->
+                  decode_bitwise'_invariant us i (Z.lor (nth_default 0 us i) (acc << nth_default 0 limb_widths i)).
   Proof.
-    induction i; intros.
-    + reflexivity.
-    + cbv [decode_bitwise'].
-      rewrite nth_default_nil, Z.shiftl_0_l.
-      apply IHi.
+    repeat match goal with
+      | |- _ => progress cbv [decode_bitwise'_invariant]; intros
+      | |- _ => erewrite testbit_bounded_high by (omega || eauto)
+      | |- _ => progress autorewrite with Ztestbit
+      | |- _ => progress rewrite sum_firstn_succ_default
+      | |- appcontext[Z.testbit _ ?n] => rewrite (Z.testbit_neg_r _ n) by omega
+      | H : forall n, 0 <= n -> Z.testbit _ n = _ |- _ => rewrite H by omega
+      | |- _ => solve [f_equal; ring]
+      | |- appcontext[Z.testbit _ (?x + sum_firstn limb_widths ?i)] =>
+        erewrite testbit_decode_digit_select with (i0 := i) by
+          (eauto; rewrite sum_firstn_succ_default; omega)
+      | |- appcontext[Z.testbit _ (?a - ?b)] => destruct (Z_lt_dec a b)
+      end.
   Qed.
 
-  Lemma decode_bitwise_nil : decode_bitwise limb_widths nil = 0.
+  Lemma decode_bitwise'_invariant_holds : forall i us acc,
+    length us = length limb_widths ->
+    bounded limb_widths us ->
+    decode_bitwise'_invariant us i acc ->
+    decode_bitwise'_invariant us 0 (decode_bitwise' limb_widths us i acc).
   Proof.
-    cbv [decode_bitwise].
-    apply decode_bitwise'_nil.
-  Qed.
-
-  Lemma decode_bitwise'_succ : forall us i acc, bounded limb_widths us ->
-    decode_bitwise' limb_widths us (S i) acc =
-    decode_bitwise' limb_widths us i (acc * (2 ^ w[i]) + nth_default 0 us i).
-  Proof.
-    intros.
-    simpl; f_equal.
-    match goal with H : bounded _ _ |- _ =>
-      rewrite Z.lor_shiftl by (auto; unfold bounded in H; specialize (H i); assumption) end.
-    rewrite Z.shiftl_mul_pow2 by auto.
-    ring.
-  Qed.
-
-  (* c is a counter, allows i to count up rather than down *)
-  Fixpoint partial_decode us i c :=
-    match c with
-    | O => 0
-    | S c' => (partial_decode us (S i) c' *  2 ^ w[i]) + nth_default 0 us i
-    end.
-
-  Lemma partial_decode_counter_over : forall c us i, (c >= length us - i)%nat ->
-    partial_decode us i c = partial_decode us i (length us - i).
-  Proof.
-    induction c; intros.
-    + f_equal. omega.
-    + simpl. rewrite IHc by omega.
-      case_eq (length us - i)%nat; intros.
-      - rewrite nth_default_out_of_bounds with (us0 := us) by omega.
-        replace (length us - S i)%nat with 0%nat by omega.
-        reflexivity.
-      - simpl. repeat f_equal. omega.
-  Qed.
-
-  Lemma partial_decode_counter_subst : forall c c' us i,
-    (c >= length us - i)%nat -> (c' >= length us - i)%nat ->
-    partial_decode us i c = partial_decode us i c'.
-  Proof.
-    intros.
-    rewrite partial_decode_counter_over by assumption.
-    symmetry.
-    auto using partial_decode_counter_over.
-  Qed.
-
-  Lemma partial_decode_succ : forall c us i, (c >= length us - i)%nat ->
-    partial_decode us (S i) c * 2 ^ w[i] + nth_default 0 us i =
-    partial_decode us i c.
-  Proof.
-    intros.
-    rewrite partial_decode_counter_subst with (i := i) (c' := S c) by omega.
-    reflexivity.
-  Qed.
-
-  Lemma partial_decode_intermediate : forall c us i, length us = length limb_widths ->
-    (c >= length us - i)%nat ->
-    partial_decode us i c = BaseSystem.decode' (base_from_limb_widths (skipn i limb_widths)) (skipn i us).
-  Proof.
-    induction c; intros.
-    + simpl. rewrite skipn_all by omega.
-      symmetry; apply decode_base_nil.
-    + simpl.
-      destruct (lt_dec i (length limb_widths)).
-      - rewrite IHc by omega.
-        do 2 (rewrite skipn_nth_default with (n := i) (d := 0) by omega).
-        unfold base_from_limb_widths; fold base_from_limb_widths.
-        rewrite peel_decode.
-        fold (BaseSystem.mul_each (two_p w[i])).
-        rewrite <-mul_each_base, mul_each_rep, two_p_correct.
-        ring_simplify.
-        f_equal; ring.
-     - rewrite <- IHc by omega.
-       apply partial_decode_succ; omega.
-  Qed.
-
-
-  Lemma decode_bitwise'_succ_partial_decode : forall us i c,
-    bounded limb_widths us -> length us = length limb_widths ->
-    decode_bitwise' limb_widths us (S i) (partial_decode us (S i) c) =
-    decode_bitwise' limb_widths us i (partial_decode us i (S c)).
-  Proof.
-    intros.
-    rewrite decode_bitwise'_succ by auto.
-    f_equal.
-  Qed.
-
-  Lemma decode_bitwise'_spec : forall us i, (i <= length limb_widths)%nat ->
-    bounded limb_widths us -> length us = length limb_widths ->
-    decode_bitwise' limb_widths us i (partial_decode us i (length us - i)) =
-    BaseSystem.decode base us.
-  Proof.
-    induction i; intros.
-    + rewrite partial_decode_intermediate by auto.
-      reflexivity.
-    + rewrite decode_bitwise'_succ_partial_decode by auto.
-      replace (S (length us - S i)) with (length us - i)%nat by omega.
-      apply IHi; auto; omega.
+    repeat match goal with
+           | |- _ => progress intros
+           | |- _ => solve [auto using decode_bitwise'_invariant_step]
+           | |- appcontext[decode_bitwise' ?a ?b ?c ?d] =>
+                functional induction (decode_bitwise' a b c d)
+            end.
   Qed.
 
   Lemma decode_bitwise_spec : forall us, bounded limb_widths us ->
     length us = length limb_widths ->
     decode_bitwise limb_widths us = BaseSystem.decode base us.
   Proof.
-    unfold decode_bitwise; intros.
-    replace 0 with (partial_decode us (length us) (length us - length us)) by
-      (rewrite Nat.sub_diag; reflexivity).
-    apply decode_bitwise'_spec; auto; omega.
+    repeat match goal with
+           | |- _ => progress cbv [decode_bitwise decode_bitwise'_invariant] in *
+           | |- _ => progress intros
+           | |- _ => rewrite sum_firstn_0
+           | |- _ => erewrite testbit_decode_high by (assumption || omega)
+           | H0 : ?P ?x , H1 : ?P ?x -> _ |- _ => specialize (H1 H0)
+           | H : _ -> forall n, 0 <= n -> Z.testbit _ n = _ |- _ => rewrite H
+           | |- decode_bitwise' ?a ?b ?c ?d = _ =>
+                  let H := fresh "H" in
+                  pose proof (decode_bitwise'_invariant_holds c b d) as H;
+                    apply Z.bits_inj'
+           | |- _ => apply Z.testbit_0_l
+           | |- _ => assumption
+           | |- _ => solve [f_equal; ring]
+           end.
   Qed.
 
 End BitwiseDecodeEncode.
@@ -622,54 +723,6 @@ Section UniformBase.
          replace x with width; try symmetry; auto.
    Qed.
 
-  Lemma decode'_tl_base_shift' : forall us lw,
-    (forall w, In w lw -> w = width) ->
-    (length us <= length lw)%nat ->
-    BaseSystem.decode' (map (Z.mul (2 ^ width)) (base_from_limb_widths lw)) us =
-    (BaseSystem.decode' (1 :: map (Z.mul (2 ^ width)) (base_from_limb_widths lw)) us) << width.
-  Proof.
-    induction us; intros ? Hin Hlength.
-    + rewrite !decode_nil, Z.shiftl_0_l; reflexivity.
-    + edestruct (destruct_repeat lw) as [? | [tl_lw [Heq_lw tl_lw_uniform]]]; eauto.
-      - subst lw; rewrite !length_cons, nil_length0 in Hlength; omega.
-      - rewrite Heq_lw in Hlength |- *.
-        rewrite base_from_limb_widths_cons, decode'_cons, two_p_correct.
-        cbv [tl].
-        fold (BaseSystem.mul_each (2 ^ width)).
-        rewrite <-!mul_each_base, !mul_each_rep.
-        rewrite decode'_cons, Z.mul_add_distr_l.
-        rewrite Z.shiftl_mul_pow2 by omega. rewrite Z.mul_add_distr_r.
-        f_equal; try ring.
-        rewrite <-Z.mul_assoc. f_equal; try ring.
-        rewrite IHus by (simpl in Hlength; auto || omega).
-        rewrite Z.shiftl_mul_pow2 by omega.
-        reflexivity.
-  Qed.
-
-  Lemma decode_tl_base_shift : forall us, (length us < length limb_widths)%nat ->
-    BaseSystem.decode (tl base) us = BaseSystem.decode base us << width.
-  Proof.
-    intros ? Hlength.
-    edestruct (destruct_repeat limb_widths) as [? | [tl_lw [Heq_lw tl_lw_uniform]]];
-        eauto; try congruence.
-    rewrite Heq_lw in Hlength |- *.
-    rewrite base_from_limb_widths_cons, two_p_correct.
-    cbv [tl].
-    apply decode'_tl_base_shift';
-      auto; simpl in *; omega.
-  Qed.
-
-  Lemma decode_shift : forall us u0, (length (u0 :: us) <= length limb_widths)%nat ->
-    BaseSystem.decode base (u0 :: us) = u0 + ((BaseSystem.decode base us) << width).
-  Proof.
-    intros.
-    rewrite <-decode_tl_base_shift by (simpl in *; omega).
-    case_eq limb_widths; try congruence; intros.
-    rewrite base_from_limb_widths_cons, decode'_cons.
-    cbv [tl].
-    f_equal; ring.
-  Qed.
-
   Lemma uniform_limb_widths_nonneg : forall w, In w limb_widths -> 0 <= w.
   Proof.
     intros.
@@ -677,8 +730,152 @@ Section UniformBase.
     replace w with width by (symmetry; auto).
     assumption.
   Qed.
+
+  (* TODO : move *)
+  Lemma decode_truncate_base : forall bs us, BaseSystem.decode bs us = BaseSystem.decode (firstn (length us) bs) us.
+  Admitted.
+
+  (* TODO : move *)
+  Lemma firstn_map : forall {A B} n (f : A -> B) ls, firstn n (map f ls) = map f (firstn n ls).
+  Proof.
+    induction n; destruct ls; boring.
+  Qed.
+  
+  (* TODO : move *)
+  Lemma firstn_base_from_limb_widths : forall n lw,
+      firstn n (base_from_limb_widths lw) = base_from_limb_widths (firstn n lw).
+  Proof.
+    induction n; destruct lw; boring.
+    f_equal.
+    rewrite <-IHn, firstn_map.
+    reflexivity.
+  Qed.
+
+  (* TODO : move *)
+  Lemma tl_repeat : forall {A} xs n (x : A), (forall y, In y xs -> y = x) ->
+                                             (n < length xs)%nat ->
+                                             firstn n xs = firstn n (tl xs).
+  Proof.
+    induction xs; destruct n; try solve [boring]; intros.
+    rewrite firstn_cons_S.
+    erewrite IHxs by (eauto using in_cons; distr_length).
+    destruct xs; distr_length.
+    cbv [tl].
+    rewrite firstn_cons_S.
+    f_equal.
+    transitivity x; [|symmetry]; eauto using in_eq, in_cons.
+  Qed.
+  
+  Lemma decode_tl_base : forall us, (length us < length limb_widths)%nat ->
+      BaseSystem.decode base us = BaseSystem.decode (base_from_limb_widths (tl limb_widths)) us.
+  Proof.
+    intros.
+    match goal with |- BaseSystem.decode ?b1 _ = BaseSystem.decode ?b2 _ => 
+      rewrite (decode_truncate_base b1), (decode_truncate_base b2) end.
+    rewrite !firstn_base_from_limb_widths.
+    do 2 f_equal.
+    eauto using tl_repeat.
+  Qed.
+
+  Lemma decode_shift_uniform : forall us u0, (length (u0 :: us) <= length limb_widths)%nat ->
+    BaseSystem.decode base (u0 :: us) = u0 + ((BaseSystem.decode base us) << width).
+  Proof.
+    intros.
+    rewrite decode_tl_base with (us := us) by distr_length.
+    rewrite decode_shift; auto using uniform_limb_widths_nonneg.
+    destruct limb_widths; try congruence;
+      repeat match goal with
+             | |- _ => rewrite base_from_limb_widths_cons
+             | |- _ => rewrite two_p_correct, Z.shiftl_mul_pow2
+             | |- _ => apply Z.add_cancel_l
+             | |- appcontext[tl (_ :: _)] => cbv [tl]
+             | |- appcontext[map (Z.mul ?a) _] => fold (BaseSystem.mul_each a);
+                                                    rewrite <-!mul_each_base, !mul_each_rep
+             | |- _ => progress distr_length
+             | |- _ => progress autorewrite with push_nth_default zsimplify
+             | |- _ => solve [auto using in_eq, Z.mul_comm]
+            end.
+    f_equal; eauto using in_eq.
+  Qed.
+
 End UniformBase.
 
+Section TestbitDecode.
+  Local Notation "u # i" := (nth_default 0 u i) (at level 30).
+
+  (* splits a bit index into a digit index and an index within the digit*)
+  Function split_index' i index lw :=
+    match lw with
+    | nil      => (index, i)
+    | w :: lw' => if Z_lt_dec i w then (index, i)
+                  else split_index' (i - w) (S index) lw'
+    end.
+
+  Lemma split_index'_ge_index : forall i index lw, (index <= fst (split_index' i index lw))%nat.
+  Proof.
+    intros; functional induction (split_index' i index lw);
+      repeat match goal with
+             | |- _ => omega
+             | |- _ => progress (simpl fst; simpl snd)
+             end.
+  Qed.
+  
+  Lemma split_index'_correct : forall i index lw,
+    sum_firstn lw (fst (split_index' i index lw) - index) + (snd (split_index' i index lw)) = i.
+  Proof.
+    intros; functional induction (split_index' i index lw);
+      repeat match goal with
+             | |- _ => omega
+             | |- _ => rewrite Nat.sub_diag
+             | |- _ => progress rewrite ?sum_firstn_nil, ?sum_firstn_0, ?sum_firstn_succ_cons
+             | |- _ => progress (simpl fst; simpl snd)
+             | |- appcontext[(fst (split_index' ?i (S ?idx) ?lw) - ?idx)%nat] =>
+               pose proof (split_index'_ge_index i (S idx) lw);
+                 replace (fst (split_index' i (S idx) lw) - idx)%nat with 
+                   (S (fst (split_index' i (S idx) lw) - S idx))%nat
+             end.
+  Qed.
+
+  Context limb_widths (limb_widths_nonneg : forall w, In w limb_widths -> 0 <= w).
+  Local Hint Resolve limb_widths_nonneg.
+  Local Notation base := (base_from_limb_widths limb_widths).
+
+  Definition split_index i := split_index' i 0 limb_widths.
+  Definition digit_index i := fst (split_index i).
+  Definition bit_index i := snd (split_index i).
+
+  Print decode_bitwise'.
+
+  Lemma testbit_decode_bitwise' : forall us i acc n,
+    length us = length limb_widths ->
+    bounded limb_widths us ->
+    Z.testbit (decode_bitwise' limb_widths us i acc) n =
+    Z.testbit (BaseSystem.decode base us) (bit_index n).
+  Proof.
+
+  SearchAbout decode_bitwise.
+  Hint Rewrite Z.testbit_0_l : Ztestbit.
+
+    Lemma testbit_decode_bitwise : forall us n,
+    length us = length limb_widths ->
+    bounded limb_widths us ->
+    Z.testbit (decode_bitwise limb_widths us) n = Z.testbit (us # digit_index n) (bit_index n).
+  Proof.
+    cbv [digit_index bit_index split_index]; induction us; intros.
+    repeat match goal with
+           | |- _ => reflexivity
+           | |- _ => progress autorewrite with Ztestbit push_nth_default
+           | |- _ => progress rewrite decode_bitwise_nil
+           end.
+    SearchAbout decode_bitwise'.
+    rewrite decode_bitwise_spec; auto.
+    rewrite decode_shift.
+    SearchAbout (BaseSystem.decode _ (_ :: _)).
+    cbv [decode_bitwise]. simpl.
+  Qed.
+
+End TestbitDecode.
+    
 Section ConversionHelper.
   Local Hint Resolve in_eq in_cons.
 
@@ -836,6 +1033,33 @@ Section Conversion.
       rewrite Z2Nat.id by (apply Z.min_case; apply dist_nonneg).
       omega.
   Defined.
+
+  Definition convert'_invariant inp i out :=
+    length out = length limb_widthsB
+    /\ forall n, Z.testbit (decodeB out) n = if Z_le_dec (Z.of_nat i) n then Z.testbit (decodeA inp) n else false.
+  
+  Lemma convert'_invariant_step : forall inp i out digitA distA digitB distB,
+    bounded limb_widthsA inp ->
+    index_and_dist i limb_widthsA = (digitA, distA) ->
+    index_and_dist i limb_widthsB = (digitB, distB) ->
+    convert'_invariant inp i out ->
+    convert'_invariant inp (i + Z.to_nat (Z.min distA distB))
+      (update_nth digitB
+         (update_by_concat_bits
+            (limb_widthsB # digitB - distB)
+            (Z.pow2_mod ((inp # digitA) >>
+             (limb_widthsA # digitA - distA)) (Z.min distA distB))) out).
+  Proof.
+    cbv [convert'_invariant]; intros; repeat pair_destruct;
+      repeat match goal with H : _ /\ _ |- _ => destruct H end;
+      repeat split.
+    + rewrite length_update_nth. assumption.
+    + intro.
+      
+
+      repeat break_if; try omega.
+      
+  Admitted.
 
   Definition convert'_invariant inp i out :=
     (i <= bitsIn limb_widthsA)%nat
